coq-verification/src/Concrete/State.v
@@ -91,7 +91,7 @@ Definition all_root_ptable_pointers {cp : concrete_params}
   : list ptable_pointer := hafnium_root_tables ++ flat_map vm_root_tables vms.
 
 Definition is_valid {cp : concrete_params} (s : concrete_state) : Prop :=
-  locations_exclusive s.(ptable_deref) all_root_ptables s.(api_page_pool)
+  locations_exclusive s.(ptable_deref) (map vm_ptable vms) hafnium_ptable s.(api_page_pool)
   (* Possible constraints:
         - Block PTEs have the valid bit set
         - page tables have a constant size
@@ -106,14 +106,14 @@ Definition vm_find {cp : concrete_params} (vid : nat) : option vm :=
 Definition vm_page_valid (s : concrete_state) (v : vm) (a : paddr_t) : Prop :=
   exists (e : pte_t) (root_ptr : ptable_pointer),
     In root_ptr v.(vm_root_tables)
-    /\ page_lookup s.(ptable_deref) root_ptr a.(pa_addr) = Some e
+    /\ page_lookup s.(ptable_deref) root_ptr Stage2 a.(pa_addr) = Some e
     /\ forall lvl, arch_mm_pte_is_valid e lvl = true.
 
 Definition haf_page_valid
            {cp : concrete_params} (s : concrete_state) (a : paddr_t) : Prop :=
   exists (e : pte_t) (root_ptr : ptable_pointer),
     In root_ptr hafnium_root_tables
-    /\ page_lookup s.(ptable_deref) root_ptr a.(pa_addr) = Some e
+    /\ page_lookup s.(ptable_deref) root_ptr Stage1 a.(pa_addr) = Some e
     /\ forall lvl, arch_mm_pte_is_valid e lvl = true.
 
 Local Definition owned (mode : mode_t) : Prop :=
@@ -122,7 +122,7 @@ Local Definition owned (mode : mode_t) : Prop :=
 Definition vm_page_owned (s : concrete_state) (v : vm) (a : paddr_t) : Prop :=
   exists (e : pte_t) (root_ptr : ptable_pointer),
     In root_ptr v.(vm_root_tables)
-    /\ page_lookup s.(ptable_deref) root_ptr a.(pa_addr) = Some e
+    /\ page_lookup s.(ptable_deref) root_ptr Stage2 a.(pa_addr) = Some e
     /\ forall lvl,
       owned (arch_mm_stage2_attrs_to_mode (arch_mm_pte_attrs e lvl)).
 
@@ -130,7 +130,7 @@ Definition haf_page_owned
            {cp : concrete_params} (s : concrete_state) (a : paddr_t) : Prop :=
   exists (e : pte_t) (root_ptr : ptable_pointer),
     In root_ptr hafnium_root_tables
-    /\ page_lookup s.(ptable_deref) root_ptr a.(pa_addr) = Some e
+    /\ page_lookup s.(ptable_deref) root_ptr Stage1 a.(pa_addr) = Some e
     /\ forall lvl,
       owned (arch_mm_stage1_attrs_to_mode (arch_mm_pte_attrs e lvl)).
 
